feat: inferFVar.WF

Lean4Lean/Verify/LocalContext.lean
@@ -1,6 +1,7 @@
 import Lean4Lean.Verify.Axioms
 import Lean4Lean.Verify.Expr
 import Lean4Lean.Verify.Typing.Expr
+import Lean4Lean.Verify.Typing.Lemmas
 
 namespace Lean.LocalContext
 
@@ -116,6 +117,62 @@ theorem mkBindingList_congr
   induction xs generalizing b <;> simp_all [mkBindingList.go]
   simp [mkBindingList1_congr H.1]
 
+inductive WF : LocalContext → Prop
+  | nil : WF ⟨.empty, .empty, .empty⟩
+  | cons :
+    d.fvarId = fv → map.find? fv = none → d.index = arr.size →
+    WF ⟨map, arr, fvmap⟩ →
+    WF ⟨map.insert fv d, arr.push d, fvmap⟩
+
+theorem WF.map_wf {lctx : LocalContext} : lctx.WF → lctx.fvarIdToDecl.WF
+  | .nil => .empty
+  | .cons _ h1 _ h2 => .insert h1 h2.map_wf
+
+theorem WF.decls_wf {lctx : LocalContext} : lctx.WF → lctx.decls.WF
+  | .nil => .empty
+  | .cons _ _ _ h2 => .push h2.decls_wf
+
+attribute [-simp] List.filterMap_reverse in
+open scoped _root_.List in
+theorem WF.map_toList : WF lctx →
+    lctx.fvarIdToDecl.toList' ~ lctx.toList.map fun d => (d.fvarId, d)
+  | .nil => by simp [LocalContext.toList]
+  | .cons h1 h2 _ h4 => by
+    subst h1; simp [LocalContext.toList]
+    exact h4.map_wf.toList'_insert _ _ (by rwa [h4.map_wf.find?_eq] at h2)
+      |>.trans (.cons _ h4.map_toList)
+
+theorem WF.find?_eq_find?_toList (H : WF lctx) :
+    lctx.find? fv = lctx.toList.find? (fv == ·.fvarId) := by
+  rw [LocalContext.find?, H.map_wf.find?_eq,
+    H.map_toList.lookup_eq H.map_wf.nodupKeys, List.map_fst_lookup]
+
+theorem WF.nodup : WF lctx → (lctx.toList.map (·.fvarId)).Nodup
+  | .nil => .nil
+  | .cons h1 h2 h3 h4 => by
+    have := h4.nodup
+    have := h4.find?_eq_find?_toList.symm.trans h2
+    simp_all [toList]
+    simpa [eq_comm] using this
+
+protected theorem WF.mkLocalDecl
+    (h1 : WF lctx) (h2 : lctx.find? fv = none) : WF (lctx.mkLocalDecl fv name ty bi kind) :=
+  .cons rfl h2 rfl h1
+
+protected theorem WF.mkLetDecl
+    (h1 : WF lctx) (h2 : lctx.find? fv = none) : WF (lctx.mkLetDecl fv name ty val bi kind) :=
+  .cons rfl h2 rfl h1
+
+@[simp] theorem mkLocalDecl_toList {lctx : LocalContext} :
+    (lctx.mkLocalDecl fv name ty bi kind).toList =
+    .cdecl lctx.decls.size fv name ty bi kind :: lctx.toList := by
+  simp [mkLocalDecl, toList]
+
+@[simp] theorem mkLetDecl_toList {lctx : LocalContext} :
+    (lctx.mkLetDecl fv name ty val bi kind).toList =
+    .ldecl lctx.decls.size fv name ty val bi kind :: lctx.toList := by
+  simp [mkLetDecl, toList]
+
 end Lean.LocalContext
 
 namespace Lean4Lean
@@ -138,63 +195,53 @@ theorem TrLocalDecl.wf : TrLocalDecl env Us Δ d d' → d'.WF env Us.length Δ.t
   | .vlam _ h | .vlet _ _ h => h
 
 variable (env : VEnv) (Us : List Name) in
-inductive TrLCtx : LocalContext → VLCtx → Prop
-  | nil : TrLCtx ⟨.empty, .empty, .empty⟩ []
+inductive TrLCtx' : List LocalDecl → VLCtx → Prop
+  | nil : TrLCtx' [] []
   | cons :
-    d.fvarId = fv → map.find? fv = none → d.index = arr.size →
-    TrLCtx ⟨map, arr, fvmap⟩ Δ → TrLocalDecl env Us Δ d d' →
-    TrLCtx ⟨map.insert fv d, arr.push d, fvmap⟩ ((some fv, d') :: Δ)
+    TrLCtx' ds Δ → TrLocalDecl env Us Δ d d' →
+    TrLCtx' (d :: ds) ((some d.fvarId, d') :: Δ)
 
-theorem TrLCtx.map_wf : TrLCtx env Us lctx Δ → lctx.fvarIdToDecl.WF
-  | .nil => .empty
-  | .cons _ h1 _ h2 _ => .insert h1 h2.map_wf
+def TrLCtx (env : VEnv) (Us : List Name) (lctx : LocalContext) (Δ : VLCtx) : Prop :=
+  lctx.WF ∧ TrLCtx' env Us lctx.toList Δ
 
-theorem TrLCtx.decls_wf : TrLCtx env Us lctx Δ → lctx.decls.WF
-  | .nil => .empty
-  | .cons _ _ _ h2 _ => .push h2.decls_wf
-
-theorem TrLCtx.noBV : TrLCtx env Us lctx Δ → Δ.NoBV
+theorem TrLCtx'.noBV : TrLCtx' env Us ds Δ → Δ.NoBV
   | .nil => rfl
-  | .cons _ _ _ h2 _ => h2.noBV
+  | .cons h _ => h.noBV
 
-theorem TrLCtx.map_toList : TrLCtx env Us lctx Δ →
-    lctx.fvarIdToDecl.toList' ~ lctx.toList.map fun d => (d.fvarId, d)
+theorem TrLCtx'.forall₂ :
+    TrLCtx' env Us ds Δ → ds.Forall₂ Δ (R := fun d d' => d'.1 = some d.fvarId)
   | .nil => by simp [LocalContext.toList]
-  | .cons h1 h2 _ h4 h5 => by
-    subst h1; simp [LocalContext.toList]
-    exact h4.map_wf.toList'_insert _ _ (by rwa [h4.map_wf.find?_eq] at h2)
-      |>.trans (.cons _ h4.map_toList)
+  | .cons h _ => by simp [LocalContext.toList]; exact h.forall₂
 
-theorem TrLCtx.forall₂ :
-    TrLCtx env Us lctx Δ → lctx.toList.Forall₂ Δ (R := fun d d' => d'.1 = some d.fvarId)
-  | .nil => by simp [LocalContext.toList]
-  | .cons h1 _ _ h4 _ => by subst h1; simp [LocalContext.toList]; exact h4.forall₂
-
-theorem TrLCtx.fvars_eq (H : TrLCtx env Us lctx Δ) : lctx.fvars = Δ.fvars := by
-  simp [LocalContext.fvars, VLCtx.fvars, LocalContext.toList]
+theorem TrLCtx'.fvars_eq (H : TrLCtx' env Us ds Δ) : ds.map (·.fvarId) = Δ.fvars := by
+  simp [VLCtx.fvars]
   induction H with
   | nil => rfl
-  | cons h1 _ _ _ _ ih => simp [h1, ← ih]
+  | cons h1 _ ih => simp [h1, ← ih]
 
-theorem TrLCtx.find?_eq_find?_toList (H : TrLCtx env Us lctx Δ) :
-    lctx.find? fv = lctx.toList.find? (fv == ·.fvarId) := by
-  rw [LocalContext.find?, H.map_wf.find?_eq,
-    H.map_toList.lookup_eq H.map_wf.nodupKeys, List.map_fst_lookup]
+theorem TrLCtx.fvars_eq (H : TrLCtx env Us lctx Δ) : lctx.fvars = Δ.fvars :=
+  H.2.fvars_eq
 
-theorem TrLCtx.find?_isSome (H : TrLCtx env Us lctx Δ) :
-    (lctx.find? fv).isSome = (Δ.find? (.inr fv)).isSome := by
-  rw [H.find?_eq_find?_toList, ← VLCtx.lookup_isSome]
-  have := H.forall₂; generalize lctx.toList = l at this ⊢; clear H
-  induction this with
+theorem TrLCtx'.find?_isSome (H : TrLCtx' env Us ds Δ) :
+    (ds.find? (fv == ·.fvarId)).isSome = (Δ.find? (.inr fv)).isSome := by
+  rw [← VLCtx.lookup_isSome]
+  induction H with
   | nil => rfl
-  | @cons d d' _ _ eq _ ih =>
-    cases d'; cases eq
+  | @cons _ _ d d' _ ih =>
     simp [List.find?, List.lookup, show (some fv == some d.fvarId) = (fv == d.fvarId) from rfl]
     split <;> simp [*]
 
+theorem TrLCtx.find?_isSome (H : TrLCtx env Us lctx Δ) :
+    (lctx.find? fv).isSome = (Δ.find? (.inr fv)).isSome := by
+  rw [H.1.find?_eq_find?_toList, H.2.find?_isSome]
+
+theorem TrLCtx'.find?_eq_some (H : TrLCtx' env Us ds Δ) :
+    (∃ d, ds.find? (fv == ·.fvarId) = some d) ↔ fv ∈ Δ.fvars := by
+  rw [← Option.isSome_iff_exists, H.find?_isSome, Option.isSome_iff_exists, VLCtx.find?_eq_some]
+
 theorem TrLCtx.find?_eq_some (H : TrLCtx env Us lctx Δ) :
     (∃ d, lctx.find? fv = some d) ↔ fv ∈ Δ.fvars := by
-  rw [← Option.isSome_iff_exists, H.find?_isSome, Option.isSome_iff_exists, VLCtx.find?_eq_some]
+  rw [H.1.find?_eq_find?_toList, H.2.find?_eq_some]
 
 theorem TrLCtx.find?_eq_none (H : TrLCtx env Us lctx Δ) :
     lctx.find? fv = none ↔ ¬fv ∈ Δ.fvars := by simp [← H.find?_eq_some]
@@ -203,19 +250,45 @@ theorem TrLCtx.contains (H : TrLCtx env Us lctx Δ) : lctx.contains fv ↔ fv �
   rw [LocalContext.contains, PersistentHashMap.find?_isSome, Option.isSome_iff_exists]
   exact H.find?_eq_some
 
-theorem TrLCtx.wf : TrLCtx env Us lctx Δ → Δ.WF env Us.length
-  | .nil => ⟨⟩
-  | .cons _ h2 _ h4 h5 => ⟨h4.wf, by simpa [← h4.find?_eq_some], h5.wf⟩
+theorem TrLCtx'.wf : TrLCtx' env Us ds Δ → (ds.map (·.fvarId)).Nodup → Δ.WF env Us.length
+  | .nil, _ => ⟨⟩
+  | .cons h1 h2, .cons H1 H2 =>
+    ⟨h1.wf H2, by simpa [← h1.find?_eq_some] using H1, h2.wf⟩
+
+theorem TrLCtx.wf (H : TrLCtx env Us lctx Δ) : Δ.WF env Us.length := H.2.wf H.1.nodup
+
+theorem TrLCtx'.find?_of_mem (henv : env.WF) (H : TrLCtx' env Us ds Δ)
+    (nd : (ds.map (·.fvarId)).Nodup) (hm : decl ∈ ds) :
+    ∃ e A, Δ.find? (.inr decl.fvarId) = some (e, A) ∧ TrExpr env Us Δ decl.type A := by
+  have := H.wf nd
+  match H with
+  | .nil => cases hm
+  | .cons (ds := ds) h1 h2 =>
+    simp [VLCtx.find?, VLCtx.next]
+    obtain _ | ⟨_, hm : decl ∈ ds⟩ := hm
+    · simp [and_assoc]
+      cases h2 with
+      | vlam h2 h3 => exact h2.weakFV henv (.skip_fvar _ _ .refl) this
+      | vlet h2 h3 => simpa [VLocalDecl.depth] using h2.weakFV henv (.skip_fvar _ _ .refl) this
+    · simp at nd; rw [if_neg (by simpa using Ne.symm (nd.1 _ hm))]; simp
+      have ⟨_, _, h1, h2⟩ := h1.find?_of_mem henv nd.2 hm
+      refine ⟨_, _, ⟨_, _, h1, rfl, rfl⟩, ?_⟩
+      simpa using h2.weakFV henv (.skip_fvar _ _ .refl) this
+
+theorem TrLCtx.find?_of_mem (henv : env.WF) (H : TrLCtx env Us lctx Δ)
+    (hm : decl ∈ lctx.toList) :
+    ∃ e A, Δ.find? (.inr decl.fvarId) = some (e, A) ∧ TrExpr env Us Δ decl.type A :=
+  H.2.find?_of_mem henv H.1.nodup hm
 
 theorem TrLCtx.mkLocalDecl
     (h1 : TrLCtx env Us lctx Δ) (h2 : lctx.find? fv = none) (h3 : TrExpr env Us Δ ty ty')
     (h4 : env.IsType Us.length Δ.toCtx ty') :
     TrLCtx env Us (lctx.mkLocalDecl fv name ty bi kind) ((some fv, .vlam ty') :: Δ) :=
-  .cons rfl h2 rfl h1 (.vlam h3 h4)
+  ⟨h1.1.mkLocalDecl h2, by simpa using .cons h1.2 (.vlam h3 h4)⟩
 
 theorem TrLCtx.mkLetDecl
     (h1 : TrLCtx env Us lctx Δ) (h2 : lctx.find? fv = none)
     (h3 : TrExpr env Us Δ ty ty') (h4 : TrExpr env Us Δ val val')
     (h5 : env.HasType Us.length Δ.toCtx val' ty') :
     TrLCtx env Us (lctx.mkLetDecl fv name ty val bi kind) ((some fv, .vlet ty' val') :: Δ) :=
-  .cons rfl h2 rfl h1 (.vlet h3 h4 h5)
+  ⟨h1.1.mkLetDecl h2, by simpa using .cons h1.2 (.vlet h3 h4 h5)⟩
